pretyping/typeclasses_errors.ml
@@ -19,13 +19,14 @@ open Nametab
 open Mod_subst
 open Topconstr
 open Util
+open Libnames
 (*i*)
 
 type contexts = Parameters | Properties
 
 type typeclass_error = 
-    | UnboundClass of identifier located
-    | UnboundMethod of identifier * identifier located (* Class name, method *)
+    | NotAClass of constr
+    | UnboundMethod of global_reference * identifier located (* Class name, method *)
     | NoInstance of identifier located * constr list
     | MismatchedContextInstance of contexts * constr_expr list * named_context (* found, expected *)
 
@@ -33,7 +34,7 @@ exception TypeClassError of env * typeclass_error
 
 let typeclass_error env err = raise (TypeClassError (env, err))
 
-let unbound_class env id = typeclass_error env (UnboundClass id)
+let not_a_class env c = typeclass_error env (NotAClass c)
 
 let unbound_method env cid id = typeclass_error env (UnboundMethod (cid, id))
 
