pretyping/typeclasses_errors.mli
@@ -19,21 +19,22 @@ open Nametab
 open Mod_subst
 open Topconstr
 open Util
+open Libnames
 (*i*)
 
 type contexts = Parameters | Properties
 
 type typeclass_error = 
-    | UnboundClass of identifier located
-    | UnboundMethod of identifier * identifier located (* Class name, method *)
+    | NotAClass of constr
+    | UnboundMethod of global_reference * identifier located (* Class name, method *)
     | NoInstance of identifier located * constr list
     | MismatchedContextInstance of contexts * constr_expr list * named_context (* found, expected *)
 
 exception TypeClassError of env * typeclass_error
 
-val unbound_class : env -> identifier located -> 'a
+val not_a_class : env -> constr -> 'a
 
-val unbound_method : env -> identifier -> identifier located -> 'a
+val unbound_method : env -> global_reference -> identifier located -> 'a
 
 val no_instance : env -> identifier located -> constr list -> 'a
 
