theories/Classes/Equivalence.v
@@ -35,16 +35,16 @@ Definition equiv [ Equivalence A R ] : relation A := R.
 
 (** Shortcuts to make proof search possible (unification won't unfold equiv). *)
 
-Program Instance [ sa : ! Equivalence A ] => equiv_refl : Reflexive equiv.
+Program Instance [ sa : ! Equivalence A ] => equiv_refl : reflexive equiv.
 
-Program Instance [ sa : ! Equivalence A ] => equiv_sym : Symmetric equiv.
+Program Instance [ sa : ! Equivalence A ] => equiv_sym : symmetric equiv.
 
   Next Obligation.
   Proof.
     symmetry ; auto.
   Qed.
 
-Program Instance [ sa : ! Equivalence A ] => equiv_trans : Transitive equiv.
+Program Instance [ sa : ! Equivalence A ] => equiv_trans : transitive equiv.
 
   Next Obligation.
   Proof.
